\documentclass[../../main.tex]{subfiles}
\newcommand{\vf}{v_F}
\allowdisplaybreaks

\begin{document}

\section{Nam form of conductivity} \label{sec:NamForm}

% !TeX spellcheck = en_GB
Starting with the form in the Nam paper, we have for the conductivity $\sigma$:
\begin{equation}
\sigma(q, \omega) = -i \frac34\frac{ n e^2}{ m} \frac{1}{\omega}\left[\int_{\Delta - \omega}^{\Delta}\dd{\omega'} \tanh(\frac{\omega + \omega'}{2T}) I_1 + \int_{\Delta}^{\infty} \dd{\omega'} \left( \tanh(\frac{\omega + \omega'}{2T}) I_1  - \tanh(\frac{\omega'}{2T})I_2 \right) \right]
\end{equation}
with 
\begin{align}
I_1 &= F(q, \Re[\sqrt{(\omega + \omega')^2 - \Delta^2} - \sqrt{\omega'^2 - \Delta^2}]) (g + 1) \nonumber\\
&\quad + F(q, \Re[-\sqrt{(\omega + \omega')^2 - \Delta^2} - \sqrt{\omega'^2 - \Delta^2}]) (g - 1) \\
I_2 &= F(q, \Re[\sqrt{(\omega + \omega')^2 - \Delta^2} - \sqrt{\omega'^2 - \Delta^2}]) (g + 1) \nonumber\\
&\quad + F(q, \Re[\sqrt{(\omega + \omega')^2 - \Delta^2} + \sqrt{\omega'^2 - \Delta^2}]) (g - 1) \\
F(q, E) &= \frac{1}{q v_0} \left[2S(E) + (1 - S(E)^2)\ln(\frac{S(E) + 1}{S(E) - 1})\right]  \\
S(E) &= \frac{1}{q v_0} \left(E - i \left( \Im[\sqrt{(\omega + \omega')^2 - \Delta^2} +\sqrt{\omega'^2 - \Delta^2}] + \frac{2}{\tau} \right) \right) \\
g  &= \frac{\omega' \left( \omega + \omega'\right) + \Delta^2}{\sqrt{\omega'^2 - \Delta^2}\sqrt{(\omega + \omega')^2 - \Delta^2}}
\end{align}

\subsection{Removing units} \label{subsec:NamForm.Dimensionless}

To remove units, we'll want to represent all the various quantities in terms of $\Delta$:
\begin{align}
\xi &= \frac{\omega}{\Delta} \\
\xi' &= \frac{\omega'}{\Delta} \\
\nu &= \frac{1}{\tau \Delta} \\
\kappa &= \frac{q v_0}{\Delta} \\
t &= \frac{T}{\Delta} \\
\sigma_0 &= \frac{n e^2}{m \Delta}
\end{align}

This gives us 
\begin{equation}
\sigma(\kappa, \xi) = -i \frac{3 \sigma_0}{4} \frac{1}{\xi}\left[\int_{1 - \xi}^{1}\dd{\xi} \tanh(\frac{\xi + \xi'}{2 t}) I_1 + \int_{1}^{\infty} \dd{\xi'} \left( \tanh(\frac{\xi + \xi'}{2t}) I_1  - \tanh(\frac{\xi'}{2t})I_2 \right) \right]
\end{equation}
with 
\begin{align}
I_1 &= F(\kappa, \Re[\sqrt{(\xi + \xi')^2 - 1} - \sqrt{\xi'^2 - 1}]) (g + 1) \nonumber\\
&\quad + F(\kappa, \Re[-\sqrt{(\xi + \xi')^2 - 1} - \sqrt{\xi'^2 - 1}]) (g - 1) \\
I_2 &= F(\kappa, \Re[\sqrt{(\xi + \xi')^2 - 1} - \sqrt{\xi'^2 - 1}]) (g + 1) \nonumber\\
&\quad + F(\kappa, \Re[\sqrt{(\xi + \xi')^2 - 1} + \sqrt{\xi'^2 - 1}]) (g - 1) \\
F(\kappa, E) &= \frac{1}{\kappa} \left[2 S(E) + (1 - S(E)^2)\ln(\frac{S(E) + 1}{S(E) - 1})\right]  \\
S(\kappa, E) &= \frac{1}{\kappa} \left(E - i \left(\Im[\sqrt{(\xi + \xi')^2 - 1} + \sqrt{\xi'^2 - 1}] + 2 \nu \right) \right) \\
g  &= \frac{\xi' \left( \xi + \xi'\right) + 1}{\sqrt{\xi'^2 - 1}\sqrt{(\xi + \xi')^2 - 1}}
\end{align}

For future reference, $F$ carried units, which when included out a $\Delta$ in the integrals.

\subsection{Comparing to normal conductivity} \label{subsec:NamForm.NormalConductivity}
We can also compare this to the normal conductivity: $\sigma_N = \frac{n e^2 \tau}{m}$:
\begin{align}
\sigma_N &= \frac{n e^2 \tau}{m} \\
&= \frac{n e^2}{m \Delta} \tau \Delta \\
&= \sigma_0 \frac{1}{\nu}
\end{align}

This, we can find the ratio $\Sigma = \frac{\sigma}{\sigma_N} = \frac{\sigma \nu}{\sigma_0}$,
\begin{equation}
\Sigma(\kappa, \xi) = -i \frac{3}{4} \frac{\nu}{\xi}\left[\int_{1 - \xi}^{1}\dd{\xi} \tanh(\frac{\xi + \xi'}{2 t}) I_1 + \int_{1}^{\infty} \dd{\xi'} \left( \tanh(\frac{\xi + \xi'}{2t}) I_1  + \tanh(\frac{\xi'}{2t})I_2 \right) \right]
\end{equation}


\end{document}
